remove unnecessary verifiability requirement for state accessors

generic/Zeta.Generic.Interleave.fst
@@ -4,6 +4,30 @@ open FStar.Classical
 open Zeta.SMap
 module SS = Zeta.SSeq
 
+//#push-options "--query_stats --debug Zeta.Generic.Interleave --debug_level SMTQuery"
+let lemma_cur_thread_state_extend (#vspec: verifier_spec) (#n:_)
+  (il: ilog vspec n) (i: seq_index il)
+  : Lemma (ensures (let st_pre = cur_thread_state_pre il i in
+                    let st_post = cur_thread_state_post il i in
+                    st_post == V.verify_step (I.index il i) st_pre))
+  = let gl = s_seq il in
+    let il_post = prefix il (i+1) in
+    interleaving_snoc il_post;
+    let t,j = i2s_map il i in
+    let tl = (t, S.index gl t) in
+    T.lemma_state_transition tl j
+//#pop-options
+
+let lemma_non_cur_thread_state_extend (#vspec: verifier_spec) (#n:_) (tid: nat{tid < n})
+  (il: ilog vspec n) (i: seq_index il)
+  : Lemma (requires (tid <> src il i))
+          (ensures (let st_pre = thread_state_pre tid il i in
+                    let st_post = thread_state_post tid il i in
+                    st_pre == st_post))
+  = let gl = s_seq il in
+    let il_post = prefix il (i+1) in
+    interleaving_snoc il_post
+
 #push-options "--fuel 0 --ifuel 1 --query_stats"
 
 let apply_per_thread_prefix (#vspec:_) (#n:_) (il: verifiable_log vspec n) (i:nat{i <= length il})
@@ -30,33 +54,27 @@ let lemma_prefix_verifiable (#vspec:_) (n:_) (il:verifiable_log vspec n) (i:nat{
     in
     forall_intro aux
 
+#pop-options
+
+let lemma_state_valid (#vspec:_) (n:_) (tid:nat{tid < n}) (il: verifiable_log vspec n)
+  : Lemma (ensures (vspec.valid (thread_state tid il)))
+  = let gl = to_glog il in
+    let tl = G.index gl tid in
+    ()
+
+let lemma_state_pre_valid (#vspec:_) (n:_) (tid:nat{tid < n}) (il: verifiable_log vspec n) (i: seq_index il)
+  : Lemma (ensures (vspec.valid (thread_state_pre tid il i)))
+  = ()
+
+let lemma_state_post_valid (#vspec:_) (n:_) (tid:nat{tid < n}) (il: verifiable_log vspec n) (i: seq_index il)
+  : Lemma (ensures (vspec.valid (thread_state_post tid il i)))
+  = ()
+
 let clock_prefix_prop (#vspec #n:_) (il: verifiable_log vspec n) (i: seq_index il) (j:nat{j <= length il /\ j > i})
   : Lemma (ensures (clock il i = clock (prefix il j) i))
   = ()
 
-//#push-options "--query_stats --debug Zeta.Generic.Interleave --debug_level SMTQuery"
-let lemma_cur_thread_state_extend (#vspec: verifier_spec) (#n:_)
-  (il: verifiable_log vspec n) (i: seq_index il)
-  : Lemma (ensures (let st_pre = cur_thread_state_pre il i in
-                    let st_post = cur_thread_state_post il i in
-                    st_post == V.verify_step (I.index il i) st_pre))
-  = let gl = to_glog il in
-    let il_post = prefix il (i+1) in
-    interleaving_snoc il_post;
-    let t,j = i2s_map il i in
-    let tl = G.index gl t in
-    T.lemma_state_transition tl j
-//#pop-options
-
-let lemma_non_cur_thread_state_extend (#vspec: verifier_spec) (#n:_) (tid: nat{tid < n})
-  (il: verifiable_log vspec n) (i: seq_index il)
-  : Lemma (requires (tid <> src il i))
-          (ensures (let st_pre = thread_state_pre tid il i in
-                    let st_post = thread_state_post tid il i in
-                    st_pre == st_post))
-  = let gl = to_glog il in
-    let il_post = prefix il (i+1) in
-    interleaving_snoc il_post
+#push-options "--fuel 0 --ifuel 1 --query_stats"
 
 let lemma_thread_state_prefix (#vspec: verifier_spec) (#n:_)
   (il: verifiable_log vspec n) (i:seq_index il)
